Added ghost methods and more predicates

Sorting/sorting.dfy
@@ -1,5 +1,41 @@
 class Sorting {
     predicate sorted(ints : seq<int>) {
-        forall i,j :: 0 <= i < j < |ints| ==> ints[i] < ints[j]
+        forall i :: 0 < i < |ints| ==> ints[i-1] < ints[i]
+    }
+
+    predicate sorted'(ints : seq<int>) {
+        forall i :: |ints| > i > 0 ==> ints[i] > ints[i-1]
+    }
+
+    predicate p(a : seq<int>, b : seq<int>) {
+        multiset(a) == multiset(b)
+    }
+
+    predicate p'(a : seq<int>, b : seq<int>) {
+        
+    }
+
+    ghost method sorted'ifsorted(ints : seq<int>)
+        requires sorted(ints)
+        ensures sorted'(ints)
+    {
+
+    }
+
+    ghost method sortedifsorted'(ints : seq<int>)
+        requires sorted'(ints)
+        ensures sorted(ints)
+    {
+
+    }
+
+    method Main() {
+        assert multiset({1, 1, 2}) == multiset{1, 2};
+        assert multiset([1, 1, 2]) == multiset([1, 2, 1]);
+
+        var m := map[];
+        m := m[1 := 3];
+        m := m[1 := m[1]+1];
+        assert m[1] == 4;
     }
 }
